an almost-proven-correct simple inode impl
one admit remaining: proving that updating a single inode in a block of inodes
does the right thing (in iput).

this inode API relies on Pack.v to update/extract inodes from a block,
and on Rec.v to convert between words on disk and the inode structure.
one of the Pack.v theorems is still unproven due to some dependent
type mess.

this inode API also doesn't yet have unified inode numbers.  instead,
inodes are identified by a tuple of (block containing the inode, offset
within that block).  i expect we should wrap iput and iget with code that
translates between flat inode numbers and these tuples, along with a proof
that the translation is a bijection, and that the representation can be
thought of as a flat list of inodes, rather than a two-dimensional list.

next, should probably implement interesting data within an inode (i.e.,
store something interesting in the inode's one-and-only data block)..

Coq bug 3731 keeps biting me, making "rewrite_strat" take forever on
certain rewrite hints, necessitating less use of "Hint Rewrite", and
explicit avoidance of "rewrite_strat" in favor of "autorewrite with core",
but that's super slow for Log.v, so we can't switch everything back to
"autorewrite with core"..

src/Inode.v
@@ -12,7 +12,7 @@ Require Import List.
 Require Import Bool.
 Require Import Eqdep_dec.
 Require Import Rec.
-Require Import AddrMap.
+Require Import Pack.
 
 Import ListNotations.
 
@@ -29,59 +29,169 @@ Record xparams := {
 Module INODE.
   Definition inodetype : Rec.rectype := [("len", addrlen); ("block0", addrlen)].
   Definition inode := Rec.recdata inodetype.
+  Definition inode_zero := Rec.word2rec inodetype $0.
 
-  Definition inode2valu (i : inode) : valu.
-    (* XXX how to convert a recdata to a word? *)
-  Admitted.
-
-  Definition valu2inode (v : valu) : inode.
-    (* XXX how to truncate the 4096-bit valu down to an inode? *)
-  Admitted.
-
-  Theorem inode2valu2inode: forall i,
-    valu2inode (inode2valu i) = i.
-  Admitted.
-
-  Definition rep xp (imap : addr -> inode) :=
-    array (IXStart xp)
-          (map (fun i => inode2valu (imap $ i)) (seq 0 (wordToNat (IXLen xp)))) $1.
-
-  Definition fupd T (m : addr -> T) a v :=
-    fun a' => if addr_eq_dec a a' then v else m a'.
-
-  Definition iget T lxp xp inum rx : prog T :=
-    v <- LOG.read_array lxp (IXStart xp) inum $1 ;
-    rx (valu2inode v).
-
-  Definition iput T lxp xp inum i rx : prog T :=
-    ok <- LOG.write_array lxp (IXStart xp) inum $1 (inode2valu i) ;
-    rx ok.
-
-  Theorem iget_ok : forall lxp xp inum,
-    {< F mbase m imap,
-    PRE    LOG.rep lxp (ActiveTxn mbase m) *
-           [[ (F * rep xp imap)%pred m ]] *
-           [[ (inum < IXLen xp)%word ]]
-    POST:r LOG.rep lxp (ActiveTxn mbase m) *
-           [[ r = imap inum ]]
-    CRASH  LOG.log_intact lxp mbase
-    >} iget lxp xp inum.
+  Definition itemsz := Rec.reclen inodetype.
+  Definition items_per_valu : addr := $32.
+  Theorem itemsz_ok : wordToNat items_per_valu * itemsz = valulen.
   Proof.
-    admit.
+    rewrite valulen_is; auto.
   Qed.
 
-  Theorem iput_ok : forall lxp xp inum i,
-    {< F mbase m imap,
+  Definition rep_block (inodes_in_block : list inode) :=
+    fold_right (fun pos v =>
+                let i := selN inodes_in_block pos inode_zero in
+                let iw := Rec.rec2word i in
+                Pack.update items_per_valu itemsz_ok v $ pos iw)
+               $0 (seq 0 (wordToNat items_per_valu)).
+
+  Definition rep xp (ilistlist : list (list inode)) :=
+    array (IXStart xp)
+          (map (fun i => rep_block (selN ilistlist i nil))
+          (seq 0 (wordToNat (IXLen xp)))) $1.
+
+  Definition iget T lxp xp iblock ipos rx : prog T :=
+    v <- LOG.read_array lxp (IXStart xp) iblock $1 ;
+    let iw := Pack.extract itemsz items_per_valu itemsz_ok v ipos in
+    let i := Rec.word2rec inodetype iw in
+    rx i.
+
+  Definition iput T lxp xp iblock ipos i rx : prog T :=
+    v <- LOG.read_array lxp (IXStart xp) iblock $1 ;
+    let iw := Rec.rec2word i in
+    let v' := Pack.update items_per_valu itemsz_ok v ipos iw in
+    ok <- LOG.write_array lxp (IXStart xp) iblock $1 v' ;
+    rx ok.
+
+  Hint Resolve Nat.lt_le_incl.
+
+  Theorem extract_sel' : forall count start ilist ipos, (ipos >= $ start)%word
+    -> (ipos < $ (start + count))%word
+    -> (start + count <= wordToNat items_per_valu)
+    -> extract itemsz items_per_valu itemsz_ok (fold_right
+         (fun (pos : nat) (v : valu) =>
+          update items_per_valu itemsz_ok v $ (pos) (Rec.rec2word (selN ilist pos inode_zero)))
+         $0 (seq start count)) ipos = Rec.rec2word (sel ilist ipos inode_zero).
+  Proof.
+    induction count; simpl; intros.
+    - exfalso. unfold not in *; apply H. replace (start) with (start+0) by omega. auto.
+    - assert (start < wordToNat items_per_valu) by ( simpl; omega ).
+      destruct (weq $ start ipos).
+      + subst. rewrite extract_same; auto.
+        unfold sel. erewrite wordToNat_natToWord_bound; eauto.
+        apply lt_wlt. erewrite wordToNat_natToWord_bound; eauto.
+      + rewrite extract_other; auto.
+        eapply IHcount; try replace (S start + count) with (start + S count) by omega; auto.
+        assert ($ start < ipos)%word by ( apply le_neq_lt; auto ).
+        unfold not; intros.
+        apply wlt_lt in H4.
+        apply wlt_lt in H3.
+        erewrite wordToNat_natToWord_bound in H3; eauto.
+        erewrite wordToNat_natToWord_bound in H4; eauto.
+        omega.
+  Qed.
+
+  Theorem extract_sel : forall ilist ipos, (ipos < items_per_valu)%word
+    -> extract itemsz items_per_valu itemsz_ok (rep_block ilist) ipos =
+       Rec.rec2word (sel ilist ipos inode_zero).
+  Proof.
+    intros; unfold rep_block.
+    apply extract_sel'.
+    intro x; apply wlt_lt in x; rewrite roundTrip_0 in *; omega.
+    rewrite plus_O_n. rewrite natToWord_wordToNat. auto.
+    omega.
+  Qed.
+
+  Hint Rewrite map_length.
+  Hint Rewrite seq_length.
+  Hint Resolve wlt_lt.
+  Hint Rewrite sel_map_seq using auto.
+  Hint Rewrite extract_sel using auto.
+  Hint Rewrite Rec.word2rec_rec2word.
+
+  Theorem iget_ok : forall lxp xp iblock ipos,
+    {< F mbase m ilistlist,
     PRE    LOG.rep lxp (ActiveTxn mbase m) *
-           [[ (F * rep xp imap)%pred m ]] *
-           [[ (inum < IXLen xp)%word ]]
+           [[ (F * rep xp ilistlist)%pred m ]] *
+           [[ (iblock < IXLen xp)%word ]] *
+           [[ (ipos < items_per_valu)%word ]]
+    POST:r LOG.rep lxp (ActiveTxn mbase m) *
+           [[ r = sel (sel ilistlist iblock nil) ipos inode_zero ]]
+    CRASH  LOG.log_intact lxp mbase
+    >} iget lxp xp iblock ipos.
+  Proof.
+    unfold iget.
+    hoare.
+
+    eexists. pred_apply. cancel.
+
+    autorewrite with core. auto.
+
+    subst. autorewrite with core. auto.
+
+    unfold LOG.log_intact; cancel.
+  Qed.
+
+  Theorem iput_ok : forall lxp xp iblock ipos i,
+    {< F mbase m ilistlist,
+    PRE    LOG.rep lxp (ActiveTxn mbase m) *
+           [[ (F * rep xp ilistlist)%pred m ]] *
+           [[ (iblock < IXLen xp)%word ]] *
+           [[ (ipos < items_per_valu)%word ]]
     POST:r ([[ r = false ]] * LOG.rep lxp (ActiveTxn mbase m)) \/
            ([[ r = true ]] * exists m', LOG.rep lxp (ActiveTxn mbase m') *
-            [[ (F * rep xp (fupd imap inum i))%pred m ]])
+            [[ (F * rep xp (upd ilistlist iblock (upd (sel ilistlist iblock nil) ipos i)))%pred m' ]])
     CRASH  LOG.log_intact lxp mbase
-    >} iput lxp xp inum i.
+    >} iput lxp xp iblock ipos i.
   Proof.
-    admit.
+    unfold iput.
+    step.
+
+    eexists. pred_apply. cancel.
+
+    autorewrite with core. auto.
+
+    (* Coq bug 3731 *)
+  intros;
+  try cancel;
+  ((eapply pimpl_ok2; [ solve [ eauto with prog ] | ])
+   || (eapply pimpl_ok2_cont; [ solve [ eauto with prog ] | | ])
+   || (eapply pimpl_ok3; [ solve [ eauto with prog ] | ])
+   || (eapply pimpl_ok3_cont; [ solve [ eauto with prog ] | | ]));
+  intros; subst;
+  try ( cancel ).
+
+    autorewrite with core in *.
+    auto.
+
+  intros;
+  try cancel;
+  ((eapply pimpl_ok2; [ solve [ eauto with prog ] | ])
+   || (eapply pimpl_ok2_cont; [ solve [ eauto with prog ] | | ])
+   || (eapply pimpl_ok3; [ solve [ eauto with prog ] | ])
+   || (eapply pimpl_ok3_cont; [ solve [ eauto with prog ] | | ]));
+  intros; subst;
+  try ( cancel ).
+
+    autorewrite with core in *.
+    apply pimpl_or_r. right.
+
+    norm.
+    cancel.
+
+    split. auto.
+    split. constructor.
+    pred_apply.
+    unfold rep.
+
+    cancel.
+
+    (* XXX *) admit.
+
+    cancel.
+
+    cancel; unfold LOG.log_intact; cancel.
+    unfold LOG.log_intact; cancel.
   Qed.
 
 End INODE.
